reconstruct stack from sets

Hoare/EvmFacts.thy
@@ -155,4 +155,561 @@ inst \<notin> {Misc STOP, Misc RETURN, Misc SUICIDE} \<union> range Unknown"
   done
 *)
 
+
+definition all :: "state_element set_pred" where
+"all s = True"
+
+definition ex :: "('a \<Rightarrow> 'b set_pred) \<Rightarrow> 'b set_pred" where
+"ex f s = (\<exists>x. f x s)"
+
+definition gas_smaller :: "int \<Rightarrow> state_element set_pred" where
+"gas_smaller x s = (\<exists>y. y < x \<and> gas_pred y s)"
+
+definition some_gas :: "state_element set_pred" where
+"some_gas s = (\<exists>y. gas_pred y s)"
+
+definition sep_add :: "'a set_pred \<Rightarrow> 'a set_pred \<Rightarrow> 'a set_pred"
+  where
+    "sep_add p q == (\<lambda> s. p s \<or> q s)"
+
+notation sep_add (infixr "##" 59)
+
+lemma sep_add_assoc [simp]: "((a ## b) ## c) = (a ## b ## c)"
+  by (simp add: sep_add_def)
+
+lemma sep_add_commute [simp]: "(a ## b)= (b ## a)"
+ by (simp add: sep_add_def) blast
+
+definition never :: "'a set_pred" where
+"never == (\<lambda>s. False)"
+
+lemma sep_add_never [simp] : "r ## never = r"
+by (simp add: never_def sep_add_def)
+
+lemma sep_add_distr [simp] : "a ** (b ## c) = a**b ## a**c"
+by (simp add: sep_def sep_add_def) blast
+
+definition failing :: "state_element set_pred" where
+"failing s = (\<exists>x. ContractActionElm (ContractFail x) \<in> s)"
+
+definition returning :: "state_element set_pred" where
+"returning s = (\<exists>x. ContractActionElm (ContractReturn x) \<in> s)"
+
+definition destructing :: "state_element set_pred" where
+"destructing s = (\<exists>x. ContractActionElm (ContractSuicide x) \<in> s)"
+
+definition calling :: "state_element set_pred" where
+"calling s = (\<exists>x. ContractActionElm (ContractCall x) \<in> s)"
+
+definition creating :: "state_element set_pred" where
+"creating s = (\<exists>x. ContractActionElm (ContractCreate x) \<in> s)"
+
+definition delegating :: "state_element set_pred" where
+"delegating s = (\<exists>x. ContractActionElm (ContractDelegateCall x) \<in> s)"
+
+lemmas rw = instruction_sem_def instruction_failure_result_def
+  subtract_gas.simps stack_2_1_op_def stack_1_1_op_def
+  stack_3_1_op_def stack_0_1_op_def  general_dup_def
+  mload_def mstore_def mstore8_def calldatacopy_def
+  codecopy_def stack_0_0_op_def jump_def jumpi_def
+  extcodecopy_def sstore_def pc_def pop_def swap_def log_def
+  stop_def create_def call_def delegatecall_def ret_def
+  suicide_def callcode_def strict_if_def blocked_jump_def
+blockedInstructionContinue_def
+
+lemma inst_no_reasons :
+"instruction_sem v c aa \<noteq>
+       InstructionToEnvironment
+        (ContractFail []) a b"
+apply (cases aa)
+apply (simp add:rw)
+apply (rename_tac inst; case_tac inst;auto simp:rw split:list.split)
+apply (rename_tac inst; case_tac inst;auto simp:rw split:list.split)
+apply (rename_tac inst; case_tac inst;auto simp:rw sha3_def
+   split:list.split if_split)
+apply(case_tac "\<not> cctx_hash_filter c ( cut_memory x21 x21a
+                (vctx_memory v))"; auto simp:rw)
+apply (rename_tac inst; case_tac inst;auto simp:rw split:list.split)
+apply (rename_tac inst; case_tac inst;
+  auto simp:rw split:list.split option.split)
+apply (rename_tac inst; case_tac inst;auto simp:rw split:list.split)
+apply (rename_tac inst; case_tac inst;auto simp:rw split:list.split)
+defer
+apply (rename_tac inst; case_tac inst;auto simp:rw split:list.split)
+apply (rename_tac inst; case_tac inst;auto simp:rw
+   split:list.split option.split)
+apply (rename_tac inst; case_tac inst;auto simp:rw split:list.split)
+apply (rename_tac inst; case_tac inst;auto simp:rw split:list.split)
+apply (rename_tac inst; case_tac inst;auto simp:rw
+   split:list.split option.split)
+apply (case_tac "vctx_next_instruction (v
+               \<lparr>vctx_stack := x22,
+                  vctx_pc := uint x21\<rparr>)
+                  c"; auto simp:rw)
+subgoal for x y aaa
+apply (case_tac aaa; auto simp:rw)
+apply (case_tac x9; auto simp:rw)
+done
+apply (case_tac "vctx_next_instruction (v
+               \<lparr>vctx_stack := x22,
+                  vctx_pc := uint x21\<rparr>)
+                  c"; auto simp:rw)
+subgoal for x y z aaa
+apply (case_tac aaa; auto simp:rw)
+apply (case_tac x9; auto simp:rw)
+done
+done
+
+lemma no_reasons_next :
+   "failed_for_reasons {}
+   (next_state stopper c (InstructionContinue v)) = False"
+apply (auto simp:failed_for_reasons_def)
+apply (cases "vctx_next_instruction v c"; auto)
+apply (auto simp:check_resources_def)
+apply (case_tac "case inst_stack_numbers aa of
+        (consumed, produced) \<Rightarrow>
+          int (length (vctx_stack v)) +
+          produced -
+          consumed
+          \<le> 1024 \<and>
+          meter_gas aa v c \<le> vctx_gas v")
+apply auto
+using inst_no_reasons apply fastforce
+using length_greater_0_conv apply fastforce
+using n_not_Suc_n apply fastforce
+done
+
+lemma program_annotation :
+"program_sem stopper c n InstructionAnnotationFailure =
+ InstructionAnnotationFailure"
+apply (induction n)
+apply (auto simp:program_sem.simps)
+done
+
+lemma program_environment :
+"program_sem stopper c n (InstructionToEnvironment a b d) =
+ (InstructionToEnvironment a b d)"
+apply (induction n)
+apply (auto simp:program_sem.simps)
+done
+
+declare next_state_def [simp del]
+
+lemma no_reasons [simp] :
+   "failed_for_reasons {}
+   (program_sem stopper c n (InstructionContinue v)) = False"
+apply (induction n arbitrary:v)
+apply (simp add:program_sem.simps failed_for_reasons_def
+  program_annotation no_reasons_next)
+apply (simp add:program_sem.simps no_reasons_next
+  failed_for_reasons_def)
+apply (case_tac "next_state stopper c
+             (InstructionContinue v)")
+using no_reasons_next
+apply force
+using program_annotation
+apply force
+using no_reasons_next 
+apply (auto simp add: program_environment failed_for_reasons_def)
+done
+
+lemmas context_rw = contexts_as_set_def constant_ctx_as_set_def variable_ctx_as_set_def
+      program_as_set_def stack_as_set_def memory_as_set_def storage_as_set_def
+      balance_as_set_def log_as_set_def data_sent_as_set_def ext_program_as_set_def
+
+lemma not_cont_insert :
+ "x (s-{ContinuingElm False}) \<Longrightarrow>
+  (x ** not_continuing) (insert (ContinuingElm False) s)"
+apply(auto simp add:rw sep_def  not_continuing_def all_def
+         failing_def some_gas_def code_def gas_pred_def context_rw)
+done
+
+lemma context_cont :
+  "contexts_as_set x1 co_ctx -
+      {ContinuingElm a, ContractActionElm b} =
+   contexts_as_set x1 co_ctx"
+apply(auto simp add:rw sep_def  not_continuing_def all_def
+         failing_def some_gas_def code_def gas_pred_def context_rw)
+done
+
+lemma context_cont1 :
+  "contexts_as_set x1 co_ctx - {ContinuingElm a} =
+   contexts_as_set x1 co_ctx"
+apply(auto simp add:rw sep_def  not_continuing_def all_def
+         failing_def some_gas_def code_def gas_pred_def context_rw)
+done
+
+lemma failing_insert :
+ "x (s-{ContractActionElm (ContractFail b)}) \<Longrightarrow>
+  (x ** failing) (insert (ContractActionElm (ContractFail b)) s)"
+apply(auto simp add:rw sep_def  not_continuing_def all_def
+         failing_def some_gas_def code_def gas_pred_def context_rw)
+done
+
+lemma some_gas_in_context :
+"(rest ** gas_pred g) s \<Longrightarrow>
+(rest ** some_gas ) s"
+apply(auto simp add:rw sep_def  not_continuing_def all_def
+         failing_def some_gas_def code_def gas_pred_def context_rw)
+done
+
+lemma case_1 :
+assumes a :
+ "(rest ** all ** code {} ** gas_pred g)
+   (contexts_as_set x1 co_ctx)"
+shows  "(rest ** not_continuing ** all ** failing ** some_gas ** code {})
+           (insert (ContinuingElm False)
+             (insert
+               (ContractActionElm (ContractFail lst))
+               (contexts_as_set x1 co_ctx)))"
+proof -
+  let ?set =  "contexts_as_set x1 co_ctx"
+  let ?base =  "rest ** all ** code {} ** some_gas"
+from a have "?base ?set"
+  by (metis set_pred.assoc some_gas_in_context)
+then have "(?base ** not_continuing) (insert (ContinuingElm False) ?set)"
+  using context_cont1 not_cont_insert by presburger
+then have "(?base ** not_continuing)
+   (insert (ContinuingElm False) ?set-{ContractActionElm (ContractFail lst)})"
+  by (metis (full_types) Diff_empty Diff_insert2 context_cont context_cont1 contexts_as_set_def insert_minus state_element.distinct(685))
+then show ?thesis
+  by (metis failing_insert insert_commute sep_three set_pred.commute) 
+qed
+
+lemma meter_gas_check :
+  "\<not> meter_gas a x1 co_ctx \<le> vctx_gas x1 \<Longrightarrow>
+   check_resources x1 co_ctx (vctx_stack x1) a \<Longrightarrow>
+   False"
+apply (simp add:check_resources_def)
+done
+
+lemmas instruction_sem_simps =
+  rw sha3_def vctx_update_storage_def
+  vctx_pop_stack_def vctx_advance_pc_def
+blockedInstructionContinue_def blocked_jump_def
+
+lemma env_meter_gas :
+"instruction_sem v1 c inst =
+ InstructionToEnvironment act v2 x33 \<Longrightarrow>
+ vctx_gas v2 = vctx_gas v1 - meter_gas inst v1 c"
+apply (simp only: instruction_sem_def)
+  apply (case_tac inst; clarsimp)
+apply (case_tac x1 ; 
+          clarsimp simp: rw
+           split:list.splits)
+         apply (case_tac x2 ; clarsimp simp: instruction_sem_simps split:list.splits)
+         apply (case_tac x3 ; clarsimp simp: instruction_sem_simps split:list.splits)
+         apply (case_tac x4 ; clarsimp simp: instruction_sem_simps split:list.splits)
+apply(case_tac "\<not> cctx_hash_filter c ( cut_memory x21 x21a (vctx_memory v1))")
+         apply (clarsimp simp: instruction_sem_simps split:list.splits)
+         apply (clarsimp simp: instruction_sem_simps split:list.splits)
+         apply (case_tac x5 ; clarsimp simp: instruction_sem_simps split:list.splits option.splits)
+         apply (case_tac x6 ; clarsimp simp: instruction_sem_simps split:list.splits option.splits)
+         apply (case_tac x7 ; clarsimp simp: instruction_sem_simps split:list.splits option.splits)
+      apply (case_tac x8 ; clarsimp simp: instruction_sem_simps Let_def split:list.splits option.splits pc_inst.splits )
+      apply (case_tac x9; clarsimp simp: instruction_sem_simps Let_def split: list.splits  pc_inst.splits option.splits)
+       apply (case_tac "x2"; clarsimp simp: instruction_sem_simps Let_def split: pc_inst.splits option.splits)
+       apply (case_tac "x21a = 0"; clarsimp simp: instruction_sem_simps Let_def split: pc_inst.splits option.splits)
+       apply (case_tac "x2"; clarsimp simp: instruction_sem_simps Let_def split: pc_inst.splits option.splits)
+       apply (case_tac "x21a = 0"; clarsimp simp: instruction_sem_simps Let_def split: pc_inst.splits option.splits)
+       apply (case_tac "x2a"; clarsimp simp: instruction_sem_simps Let_def split: pc_inst.splits option.splits)
+     apply (case_tac "x10"; clarsimp simp: instruction_sem_simps  split: pc_inst.splits option.splits list.splits)
+     apply (clarsimp simp: instruction_sem_simps  split: pc_inst.splits option.splits)
+     apply (case_tac "x12"; clarsimp simp: instruction_sem_simps Let_def split: pc_inst.splits option.splits)
+     apply (case_tac "x13"; clarsimp simp: instruction_sem_simps  split: pc_inst.splits option.splits list.splits if_splits)
+done
+
+lemma continue_meter_gas :
+"instruction_sem v1 c inst =
+ InstructionContinue v2 \<Longrightarrow>
+ vctx_gas v2 = vctx_gas v1 - meter_gas inst v1 c"
+apply (simp only: instruction_sem_def)
+  apply (case_tac inst; clarsimp)
+apply (case_tac x1 ; 
+          clarsimp simp: rw
+           split:list.splits)
+         apply (case_tac x2 ; clarsimp simp: instruction_sem_simps split:list.splits)
+         apply (case_tac x3 ; clarsimp simp: instruction_sem_simps split:list.splits)
+         apply (case_tac x4 ; clarsimp simp: instruction_sem_simps split:list.splits)
+apply(case_tac "\<not> cctx_hash_filter c ( cut_memory x21 x21a (vctx_memory v1))")
+         apply (clarsimp simp: instruction_sem_simps split:list.splits)
+         apply (clarsimp simp: instruction_sem_simps split:list.splits)
+         apply (case_tac x5 ; clarsimp simp: instruction_sem_simps split:list.splits option.splits)
+         apply (case_tac x6 ; clarsimp simp: instruction_sem_simps split:list.splits option.splits)
+         apply (case_tac x7 ; clarsimp simp: instruction_sem_simps split:list.splits option.splits)
+      apply (case_tac x8 ; clarsimp simp: instruction_sem_simps Let_def split:list.splits option.splits pc_inst.splits )
+      apply (case_tac x9; clarsimp simp: instruction_sem_simps Let_def split: list.splits  pc_inst.splits option.splits)
+       apply (case_tac "x2"; clarsimp simp: instruction_sem_simps Let_def split: pc_inst.splits option.splits)
+       apply (case_tac "x21a = 0"; clarsimp simp: instruction_sem_simps Let_def split: pc_inst.splits option.splits)
+       apply (case_tac "x2"; clarsimp simp: instruction_sem_simps Let_def split: pc_inst.splits option.splits)
+       apply (case_tac "x21a = 0"; clarsimp simp: instruction_sem_simps Let_def split: pc_inst.splits option.splits)
+       apply (case_tac "x2a"; clarsimp simp: instruction_sem_simps Let_def split: pc_inst.splits option.splits)
+     apply (case_tac "x10"; clarsimp simp: instruction_sem_simps  split: pc_inst.splits option.splits list.splits)
+     apply (clarsimp simp: instruction_sem_simps  split: pc_inst.splits option.splits)
+     apply (case_tac "x12"; clarsimp simp: Let_def instruction_sem_simps  split: pc_inst.splits option.splits)
+     apply (case_tac "x13"; clarsimp simp: instruction_sem_simps  split: pc_inst.splits option.splits list.splits if_splits)
+done
+
+lemma no_annotation_inst :
+"instruction_sem v c a \<noteq> InstructionAnnotationFailure"
+apply (cases a)
+apply (simp add:rw)
+apply (rename_tac inst; case_tac inst;auto simp:rw split:list.split)
+apply (rename_tac inst; case_tac inst;auto simp:rw split:list.split)
+apply (rename_tac inst; case_tac inst;auto simp:rw sha3_def
+   split:list.split if_split)
+apply(case_tac "\<not> cctx_hash_filter c ( cut_memory x21 x21a
+                (vctx_memory v))"; auto simp:rw)
+apply (rename_tac inst; case_tac inst;auto simp:rw split:list.split)
+apply (rename_tac inst; case_tac inst;
+  auto simp:rw split:list.split option.split)
+apply (rename_tac inst; case_tac inst;auto simp:rw split:list.split)
+apply (rename_tac inst; case_tac inst;auto simp:rw split:list.split)
+defer
+apply (rename_tac inst; case_tac inst;auto simp:rw split:list.split)
+apply (rename_tac inst; case_tac inst;auto simp:rw
+   split:list.split option.split)
+apply (rename_tac inst; case_tac inst;auto simp:rw split:list.split)
+apply (rename_tac inst; case_tac inst;auto simp:rw split:list.split)
+apply (rename_tac inst; case_tac inst;auto simp:rw
+   split:list.split option.split)
+apply (case_tac "vctx_next_instruction (v
+               \<lparr>vctx_stack := x22,
+                  vctx_pc := uint x21\<rparr>)
+                  c"; auto simp:rw)
+subgoal for x y aaa
+apply (case_tac aaa; auto simp:rw)
+apply (case_tac x9; auto simp:rw)
+done
+apply (case_tac "vctx_next_instruction (v
+               \<lparr>vctx_stack := x22,
+                  vctx_pc := uint x21\<rparr>)
+                  c"; auto simp:rw)
+subgoal for x y z aaa
+apply (case_tac aaa; auto simp:rw)
+apply (case_tac x9; auto simp:rw)
+done
+done
+
+lemma call_instruction :
+"instruction_sem v c inst =
+ InstructionToEnvironment (ContractCall args) x32 x33 \<Longrightarrow>
+ inst = Misc CALL \<or> inst = Misc CALLCODE"
+apply (simp only: instruction_sem_def)
+  apply (case_tac inst; clarsimp)
+apply (case_tac x1 ; 
+          clarsimp simp: rw
+           split:list.splits)
+         apply (case_tac x2 ; clarsimp simp: instruction_sem_simps split:list.splits)
+         apply (case_tac x3 ; clarsimp simp: instruction_sem_simps split:list.splits)
+         apply (case_tac x4 ; clarsimp simp: instruction_sem_simps split:list.splits)
+apply(case_tac "\<not> cctx_hash_filter c ( cut_memory x21 x21a (vctx_memory v))")
+         apply (clarsimp simp: instruction_sem_simps split:list.splits)
+         apply (clarsimp simp: instruction_sem_simps split:list.splits)
+         apply (case_tac x5 ; clarsimp simp: instruction_sem_simps split:list.splits option.splits)
+         apply (case_tac x6 ; clarsimp simp: instruction_sem_simps split:list.splits option.splits)
+         apply (case_tac x7 ; clarsimp simp: instruction_sem_simps split:list.splits option.splits)
+      apply (case_tac x8 ; clarsimp simp: instruction_sem_simps Let_def split:list.splits option.splits pc_inst.splits )
+      apply (case_tac x9; clarsimp simp: instruction_sem_simps Let_def split: list.splits  pc_inst.splits option.splits)
+       apply (case_tac "x2"; clarsimp simp: instruction_sem_simps Let_def split: pc_inst.splits option.splits)
+       apply (case_tac "x21a = 0"; clarsimp simp: instruction_sem_simps Let_def split: pc_inst.splits option.splits)
+       apply (case_tac "x2"; clarsimp simp: instruction_sem_simps Let_def split: pc_inst.splits option.splits)
+       apply (case_tac "x21a = 0"; clarsimp simp: instruction_sem_simps Let_def split: pc_inst.splits option.splits)
+       apply (case_tac "x2a"; clarsimp simp: instruction_sem_simps Let_def split: pc_inst.splits option.splits)
+     apply (case_tac "x10"; clarsimp simp: instruction_sem_simps  split: pc_inst.splits option.splits list.splits)
+     apply (clarsimp simp: instruction_sem_simps  split: pc_inst.splits option.splits)
+     apply (case_tac "x12"; clarsimp simp: Let_def instruction_sem_simps  split: pc_inst.splits option.splits)
+     apply (case_tac "x13"; clarsimp simp: instruction_sem_simps  split: pc_inst.splits option.splits list.splits if_splits)
+done
+
+lemma call_decr_gas :
+   assumes a:"instruction_sem v1 co_ctx a =
+       InstructionToEnvironment (ContractCall x1a)
+        v2 x33"
+   and good:"vctx_memory_usage v1 \<ge> 0"
+  shows  "vctx_gas v1 \<ge> vctx_gas v2"
+proof -
+  have inst: "a = Misc CALL \<or> a = Misc CALLCODE"
+   using call_instruction and a by force
+  then have "meter_gas a v1 co_ctx > 0"
+   using good and meter_gas_gt_0 by blast
+  then show ?thesis using env_meter_gas and a by force
+qed
+
+(* Perhaps "all" will have to hog absolutely everything
+ ??? *)
+
+(*
+lemma gas_decreases_in_triples :
+ "g1 \<ge> g2 \<Longrightarrow>
+  GasElm g1 \<in> s1 \<Longrightarrow>
+  GasElm g2 \<in> s2 \<Longrightarrow>
+  (\<forall>h1. GasElm h1 \<in> s1 \<longrightarrow> h1 = g1) \<Longrightarrow>
+  (\<forall>h2. GasElm h2 \<in> s2 \<longrightarrow> h2 = g2) \<Longrightarrow>
+  (all ** gas_pred g) s1 \<Longrightarrow>
+  (all ** gas_smaller g) s2"
+apply(auto simp add:rw sep_def gas_smaller_def  not_continuing_def all_def
+         failing_def some_gas_def code_def gas_pred_def context_rw)
+*)
+
+(* need to make a better 'all' should have a feature
+   like this *)
+
+definition all_stack :: "state_element set_pred" where
+"all_stack s = (\<exists>t. s = stack_as_set t)"
+
+definition all_but_gas :: "state_element set_pred" where
+"all_but_gas s = (\<exists>c v.
+   s = contexts_as_set v c - {GasElm (vctx_gas v)})"
+
+lemma maximality_stack_aux :
+   "stack_as_set s1 \<subseteq> stack_as_set s2 \<Longrightarrow>
+    i < length s1 \<Longrightarrow>
+    rev s1!i = rev s2!i"
+apply(auto simp add:context_rw)
+apply blast
+done
+
+lemma maximality_stack_length :
+   "stack_as_set s1 \<subseteq> stack_as_set s2 \<Longrightarrow>
+    length s1 = length s2"
+by (auto simp add:context_rw)
+
+lemma list_eq :
+   "length l1 = length l2 \<Longrightarrow>
+    (\<forall>i. i < length l1 \<longrightarrow> l1!i = l2!i) \<Longrightarrow>
+    rev l1 = rev l2"
+apply (rule List.nth_equalityI)
+apply auto
+  by (simp add: Suc_diff_Suc rev_nth)
+
+
+lemma maximality_stack_aux2 :
+ "stack_as_set s1 \<subseteq> stack_as_set s2 \<Longrightarrow>
+  rev s1 = rev s2"
+apply (rule list_eq)
+using maximality_stack_length
+apply force
+apply auto
+subgoal for i
+using maximality_stack_aux [of s1 s2 "length s2 - i -1"]
+  and maximality_stack_length [of s1 s2]
+proof -
+  assume a1: "i < length s1"
+  assume a2: "stack_as_set s1 \<subseteq> stack_as_set s2"
+  have f3: "\<not> stack_as_set s1 \<subseteq> stack_as_set s2 \<or> length s1 = length s2"
+    by (metis \<open>stack_as_set s1 \<subseteq> stack_as_set s2 \<Longrightarrow> length s1 = length s2\<close>)
+  have f4: "length s2 - i - 1 = length s2 - Suc i"
+    using diff_Suc_eq_diff_pred diff_commute by presburger
+  have "0 < length s2"
+    using f3 a2 a1 by linarith
+  then have "rev s1 ! (length s2 - i - 1) = rev s2 ! (length s2 - i - 1)"
+    using f4 f3 a2 \<open>\<lbrakk>stack_as_set s1 \<subseteq> stack_as_set s2; length s2 - i - 1 < length s1\<rbrakk> \<Longrightarrow> rev s1 ! (length s2 - i - 1) = rev s2 ! (length s2 - i - 1)\<close> diff_Suc_less by presburger
+  then show ?thesis
+    using f4 f3 a2 a1 by (metis (no_types) nth_rev_alt)
+qed
+done
+
+lemma maximality_stack :
+ "stack_as_set s1 \<subseteq> stack_as_set s2 \<Longrightarrow>
+  s1 = s2"
+using maximality_stack_aux2
+  by auto
+
+lemma stack_height_at_context :
+ "StackHeightElm x \<in> contexts_as_set v2 c2 \<Longrightarrow>
+  StackHeightElm x \<in> stack_as_set (vctx_stack v2)"
+apply(simp add:context_rw)
+done
+
+lemma stack_elem_at_context :
+ "StackElm (x,y) \<in> contexts_as_set v2 c2 \<Longrightarrow>
+  StackElm (x,y) \<in> stack_as_set (vctx_stack v2)"
+apply(simp add:context_rw)
+done
+
+lemma stack_at_context :
+ "stack_as_set s1 \<subseteq> contexts_as_set v2 c2 \<Longrightarrow>
+  stack_as_set s1 \<subseteq> stack_as_set (vctx_stack v2)"
+apply auto
+apply (case_tac x)
+apply auto
+using stack_height_at_context
+apply force
+using stack_elem_at_context
+apply force
+apply(auto simp add:context_rw)
+done
+
+lemma stack_from_context :
+ "stack_as_set s1 \<subseteq> contexts_as_set v2 c2 \<Longrightarrow>
+  vctx_stack v2 = s1"
+using stack_at_context [of s1 v2 c2]
+  and maximality_stack [of s1 "vctx_stack v2"]
+by force
+
+lemma maximality_data_aux :
+   "data_sent_as_set s1 \<subseteq> data_sent_as_set s2 \<Longrightarrow>
+    i < length s1 \<Longrightarrow>
+    s1!i = s2!i"
+apply(auto simp add:context_rw)
+apply blast
+done
+
+lemma maximality_data_length :
+   "data_sent_as_set s1 \<subseteq> data_sent_as_set s2 \<Longrightarrow>
+    length s1 = length s2"
+by (auto simp add:context_rw)
+
+lemma maximality_data_sent :
+ "data_sent_as_set s1 \<subseteq> data_sent_as_set s2 \<Longrightarrow>
+  s1 = s2"
+apply (rule List.nth_equalityI)
+using maximality_data_length
+apply force
+apply auto
+subgoal for i
+using maximality_data_aux [of s1 s2 i]
+apply simp
+done
+done
+
+lemma data_size_at_context :
+ "SentDataLengthElm x \<in> contexts_as_set v2 c2 \<Longrightarrow>
+  SentDataLengthElm x \<in> data_sent_as_set (vctx_data_sent v2)"
+apply(simp add:context_rw)
+done
+
+lemma data_elem_at_context :
+ "SentDataElm (x,y) \<in> contexts_as_set v2 c2 \<Longrightarrow>
+  SentDataElm (x,y) \<in> data_sent_as_set (vctx_data_sent v2)"
+apply(simp add:context_rw)
+done
+
+lemma data_at_context :
+ "data_sent_as_set s1 \<subseteq> contexts_as_set v2 c2 \<Longrightarrow>
+  data_sent_as_set s1 \<subseteq> data_sent_as_set (vctx_data_sent v2)"
+apply (auto)
+apply (case_tac x)
+apply (auto simp:data_size_at_context data_elem_at_context)
+apply(auto simp add:context_rw)
+done
+
+lemma data_from_context :
+ "data_sent_as_set s1 \<subseteq> contexts_as_set v2 c2 \<Longrightarrow>
+  vctx_data_sent v2 = s1"
+using data_at_context [of s1 v2 c2]
+  and maximality_data_sent [of s1 "vctx_data_sent v2"]
+by force
+
+
+(*
+lemma maximality :
+   "contexts_as_set v1 c1 \<subseteq> contexts_as_set v2 c2 \<Longrightarrow>
+    a \<in> contexts_as_set v2 c2 \<Longrightarrow>
+    a \<in> contexts_as_set v1 c1"
+apply(simp add:context_rw)
+apply clarsimp
+*)
+
 end
